range1.bpl
@@ -1,0 +1,113 @@
+//type Ref is intended to represent object references
+type Ref;
+type PredicateTypes;
+type FractionType = [Ref] int;
+type PackedType = [Ref, PredicateTypes] bool;
+
+const null:Ref;
+const unique RangeP:PredicateTypes;
+
+var val: [Ref]int;
+var next: [Ref]Ref;
+
+var fracRangeP: FractionType;
+var packed: PackedType;
+
+//global variables that keep track of the parameters of the Range predicate
+//that are not values of fields
+var xRangePred: [Ref] int;
+var yRangePred: [Ref] int;
+
+procedure ConstructRange0(this: Ref, v: int, n: Ref);
+	ensures (val[this] == v) && 
+		(next[this] == n) && 
+		(packed[this, RangeP]) && 
+		(fracRangeP[this] >= 100);
+
+//after calling procedures PackRangeNextNull, any kind 
+//of Pack procedures, I have to do
+//packed[this, rangeP]:=true
+
+//Boogie code needs to be much closer to the Java code. 
+//We do not want PackRangeNextNull and PackRangeNextNotNull.
+//We only want one PackRange.
+
+//Isn't this != null implied?
+procedure PackRange(this:Ref, x:int, y:int);
+	requires (this != null) && 
+		 (val[this] >= x) &&
+		 (val[this] <= y) &&
+		 ( (next[this] == null) || 
+		 	(packed[next[this], RangeP] &&
+			(fracRangeP[next[this]] >= 1) &&
+			(xRangePred[next[this]] == x) && 
+			(yRangePred[next[this]] == y))
+		 );
+	ensures (xRangePred[this]==x) && (yRangePred[this]==y);
+	//Might need to do the above ensures in an assignment instead?
+
+
+procedure UnpackRange(this:Ref, x:int, y:int);
+	requires packed[this, RangeP] && 
+		(xRangePred[this]==x) &&
+		(yRangePred[this]==y) &&
+		(fracRangeP[this] >= 1);
+	ensures (this != null) && 
+		 (val[this] >= x) &&
+		 (val[this] <= y) &&
+		 ( (next[this] == null) || 
+		 	(packed[next[this], RangeP] &&
+			(fracRangeP[next[this]] >= 1) &&
+			(xRangePred[next[this]] == x) && 
+			(yRangePred[next[this]] == y))
+		 );
+ 
+
+//modulo is not implemented in Boogie
+//so its properties have to be described  
+function modulo(x:int, y:int) returns (int);
+  axiom (forall x:int, y:int :: {modulo(x,y)} 
+    ((0<=x) &&(0<y) ==> (0<= modulo(x,y) ) && (modulo(x,y)<y) )
+    &&
+    ((0<=x) &&(y<0) ==> (0<= modulo(x,y) ) && (modulo(x,y)<-y) )
+    &&
+    ((x<=0) &&(0<y) ==> (-y<= modulo(x,y) ) && (modulo(x,y)<=0) )
+    &&
+    ((x<=0) &&(y<0) ==> (y<= modulo(x,y) ) && (modulo(x,y)<=0) )
+   );    
+
+procedure addModulo11(this: Ref, x:int) 
+modifies val, packed, xRangePred, fracRangeP;
+//need to put this in for modulo 
+requires this!=null;
+//requires x>=0;
+//this could be 100 here
+//requires fracRangeP[this]>=50;
+requires xRangePred[this]==0; 
+requires yRangePred[this]==10;
+requires packed[this, RangeP];
+ensures packed[this, RangeP];
+ensures xRangePred[this]==0; 
+ensures yRangePred[this]==10;
+//ensures fracRangeP[this]>=50;
+{
+//We need to be careful about assumes.
+//And use them sparingly.
+call UnpackRange(this, 0, 10);
+packed[this, RangeP]:=false;
+
+val[this] := modulo((val[this]+x),11);
+
+if (next[this] != null )
+  { 
+call addModulo11(next[this], x);
+  }
+
+  //val[this] was not modified
+  //but Boogie does not know that
+
+call PackRange(this, 0, 10);
+
+call PackRange(this, 0, 10);
+packed[this,RangeP]:=true;
+  }
